fixes

playground/uart_model/nit2bisim/nit2bisim2Script.sml
@@ -3,28 +3,44 @@
          loadPath := ("../prog"::(!loadPath));
          loadPath := ("../clock"::(!loadPath));
  *)
+
 open HolKernel Parse boolLib bossLib;
 open m0_NITTheory
 open uartTheory
-open m0u_progTheory
-open m0_progTheory
+open pairTheory;
+open progTheory;
+open m0u_progTheory;
+open set_sepTheory;
+open m0_NITTheory;
+open m0_progTheory;
+open uartTheory
+open clockTheory;
 open stateTheory m0_stepTheory;
 open boolSimps;
 open pred_setTheory;
-open m0_progTheory;
-open pairTheory;
-open progTheory;
-open set_sepTheory;
-open clockTheory;
+
+
+
 
 val _ = new_theory "nit2bisim2";
 
+
+fun rm_assum pat = Q.PAT_X_ASSUM pat (fn x => ALL_TAC );
 (********************************************)
 (*          No exceptions                   *)
 (*                                          *)
 (********************************************)
 
-(* There will be no exceptions for t clock 
+
+val SEQ_MONO_LEM = Q.prove( `!seq s i t.
+    (rel_sequence (NEXT_REL $= NextStateM0) seq s)/\
+    ((seq (SUC i)).count < s.count + t)==> ((seq i).count < s.count + t)`,
+    REPEAT GEN_TAC>>
+    (MP_TAC o Q.SPECL[`s`,`i`,`SUC i`,`seq`] ) SEQ_MONO_B>>
+    ASM_SIMP_TAC std_ss []>>
+    METIS_TAC [ DECIDE ``( x:num <= y:num /\ y < z:num ) ==> (x < z) ``]
+);
+(* will be no exceptions for t clock 
    cycles executing from a state constrained by P *)
 
 val NEX_def = Define `
@@ -34,84 +50,6 @@ val NEX_def = Define `
                ((seq (i)).count < s.count+ t))==>   
 	           ((seq i).count < (Next(seq i)).count) /\
                    ((Next (seq (i))).exception = NoException) `;
-
-val NEX_VERI_0_thm= Q.store_thm("NEX_VERI_0_thm",
-`!P. NEX P 0`,
-    fs[NEX_def]>>
-    REPEAT strip_tac>>
-    (`(s).count ≤ (seq i).count` by
-        METIS_TAC[SEQ_MONO_B, DECIDE ``0n<=i``, 
-                  rel_sequence_def, NEXT_REL_def,
-                  NextStateM0_def]
-        )>>
-    fs[]
-);
-
-
-
-(* This is our strong non interference property
-   After executing t clock cycles no information flow to or from the region can be observed
-   in each step
-*)
-val NIT_def = Define`
-NIT region(P :(m0_component # m0_data -> bool) -> bool)  t =   !s s' seq seq' i.   
-               ((SEP_REFINE (P * SEP_T) ($=) (STATE m0_proj) s) /\
-               m0_non_r_eq region s s' /\ 
-               rel_sequence (NEXT_REL $= NextStateM0) seq  s /\
-               rel_sequence (NEXT_REL $= NextStateM0) seq' s' /\
-               ((seq i).count < s.count+t)) ==>   
-                   m0_non_r_eq region (seq (SUC i)) (seq' (SUC i)) /\
-                   m0_r_eq region (seq' 0) (seq' (SUC i))
-`;
-
-
-
-
-val NIT_NIT_STEP_thm = store_thm("NIT_NIT_STEP_thm",
-``  ! P t region. 
-        ((NEX P t)/\ (NIT region P t)) = ! s seq i . (
-        SEP_REFINE (P * SEP_T) $= (STATE m0_proj) s /\
-        rel_sequence (NEXT_REL $= NextStateM0) seq s /\
-        (seq i).count < s.count + t ==> NIT_STEP region (seq i))``,
-        cheat
-);
-
-(* bisim *)
-val SEQ_MONO_LEM = Q.prove( `!seq s i t.
-    (rel_sequence (NEXT_REL $= NextStateM0) seq s)/\
-    ((seq (SUC i)).count < s.count + t)==> ((seq i).count < s.count + t)`,
-    REPEAT GEN_TAC>>
-    (MP_TAC o Q.SPECL[`s`,`i`,`SUC i`,`seq`] ) SEQ_MONO_B>>
-    ASM_SIMP_TAC std_ss []>>
-    METIS_TAC [ DECIDE ``( x:num <= y:num /\ y < z:num ) ==> (x < z) ``]
-);
-
-val COSIM'_def = Define `COSIM' P t = ! s s' seq seq' i.
-    ((SEP_REFINE (P * SEP_T) ($=) (STATE m0_proj) s) /\
-    rel_sequence (NEXT_REL $= NextStateM0) seq  s /\
-    rel_sequence (NEXT_REL $= NextStateM0U) seq' s' /\
-    m0u_m0_non_r_eq uart_r s' s /\ ((seq i).count < s.count + t) )==>
-        m0u_m0_non_r_eq uart_r (m0u_Next (seq' i)) (Next (seq i)) /\
-        m0u_r_eq uart_r (seq' i)  (m0u_Next (seq' i))`;
-
-val COSIM''_def = Define `COSIM'' P t = ! s s' seq seq' i.
-    ((SEP_REFINE (P * SEP_T) ($=) (STATE m0_proj) s) /\
-    rel_sequence (NEXT_REL $= NextStateM0) seq  s /\
-    rel_sequence (NEXT_REL $= NextStateM0U) seq' s' /\
-    m0u_m0_non_r_eq uart_r s' s /\ ((seq i).count < s.count + t) )==>
-        m0u_m0_non_r_eq uart_r (seq' (SUC i)) (seq (SUC i)) /\
-        m0u_r_eq uart_r (seq' i)  (seq' (SUC i))`;
-
-val COSIM_def = Define `COSIM P t = ! s s' seq seq' i.
-    ((SEP_REFINE (P * SEP_T) ($=) (STATE m0_proj) s) /\
-    rel_sequence (NEXT_REL $= NextStateM0) seq  s /\
-    rel_sequence (NEXT_REL $= NextStateM0U) seq' s' /\
-    m0u_m0_non_r_eq uart_r s' s /\ ((seq i).count <= s.count + t) )==>
-        m0u_m0_non_r_eq uart_r (seq' ( i)) (seq ( i)) /\
-        m0u_r_eq uart_r (seq' 0)  (seq' ( i))`;
-
-
-val cosim_def = Define `cosim P c t = COSIM ((CODE_POOL m0_instr c) * P  ) t`;
 
 val NEX_thm = Q.store_thm("NEX_thm",
     `! P t s seq i. 
@@ -138,24 +76,299 @@ val NEX_thm = Q.store_thm("NEX_thm",
     METIS_TAC[]
 );
 
-val PRODUCT_STATE_lem = prove(``!s z_i. ?z_0. m0_non_r_eq uart_r s z_0 /\ m0_r_eq uart_r z_0 z_i``,
-    REPEAT GEN_TAC>>
-    EXISTS_TAC ``s with <|MEM := (\x. if (x IN uart_r)
-                                         then (z_i.MEM x)
-                                         else (s.MEM x)) |>``>>
-    SIMP_TAC (std_ss++pred_setLib.PRED_SET_ss) [m0Theory.m0_state_accfupds,
-                m0_non_r_eq_def, m0_r_eq_def, mem_eq_def]
+val NEX_VERI_0_thm= Q.store_thm("NEX_VERI_0_thm",
+`!P. NEX P 0`,
+    fs[NEX_def]>>
+    REPEAT strip_tac>>
+    (`(s).count ≤ (seq i).count` by
+        METIS_TAC[SEQ_MONO_B, DECIDE ``0n<=i``, 
+                  rel_sequence_def, NEXT_REL_def,
+                  NextStateM0_def]
+        )>>
+    fs[]
 );
+
+val VC_def = Define`
+VC region(P :(m0_component # m0_data -> bool) -> bool)  t =   !s s' seq seq' i.   
+               ((SEP_REFINE (P * SEP_T) ($=) (STATE m0_proj) s) /\
+               m0_non_r_eq region s s' /\ 
+               rel_sequence (NEXT_REL $= NextStateM0) seq  s /\
+               rel_sequence (NEXT_REL $= NextStateM0) seq' s' /\
+               ((seq i).count < s.count+t)) ==>   
+                   m0_non_r_eq region (seq (SUC i)) (seq' (SUC i)) /\
+                   m0_r_eq region (seq' 0) (seq' (SUC i))
+`;
+
+(* This is our strong non interference property
+   After executing t clock cycles no information flow to or from the region can be observed
+   in each step
+*)
 
 val eq_lem = prove(``!a b r.
     m0_non_r_eq r a  b /\ m0_r_eq r a b ==> (a=b)``,
-
     REPEAT GEN_TAC>>
     Cases_on `a`>>Cases_on `b`>>
     SIMP_TAC (std_ss++pred_setLib.PRED_SET_ss) [m0Theory.m0_state_accfupds,
-m0Theory.m0_state_accessors,m0_non_r_eq_def, m0_r_eq_def, mem_eq_def, m0Theory.m0_state_11]>>
+            m0Theory.m0_state_accessors,m0_non_r_eq_def, m0_r_eq_def, mem_eq_def, m0Theory.m0_state_11]>>
     Cases_on  `x NOTIN r ` >> METIS_TAC[]
 );
+
+val PRODUCT_STATE_lem = prove(``!s z_i. ?z_0. m0_non_r_eq uart_r s z_0 /\ m0_r_eq uart_r z_0 z_i``,
+    REPEAT GEN_TAC>>
+    EXISTS_TAC ``s with <|MEM := (\x. if (x IN uart_r) 
+                                         then (z_i.MEM x)
+                                         else (s.MEM x)) |>``>>
+    SIMP_TAC (std_ss++pred_setLib.PRED_SET_ss) [m0Theory.m0_state_accfupds,
+		m0_non_r_eq_def, m0_r_eq_def, mem_eq_def]
+);
+
+val VC_WEAKEN_lem = prove(
+    ``! P t t' uart_r.
+         (VC uart_r P t) /\ 
+         (t' <= t)  
+          ==> VC uart_r P t'``,
+    SIMP_TAC std_ss [VC_def]>>
+    REPEAT STRIP_TAC>>
+    `(seq i).count < s.count + t` by DECIDE_TAC>>
+    METIS_TAC []
+);
+
+val NEX_WEAKEN_lem = prove(
+    ``! P t t' uart_r.
+         (NEX P t) /\ 
+         (t' <= t)  
+          ==> NEX P t'``,
+    SIMP_TAC std_ss [NEX_def]>>
+    REPEAT STRIP_TAC>>
+    `(seq i).count < s.count + t` by DECIDE_TAC>>
+    METIS_TAC []
+);
+
+val m0_non_r_eq_lem = prove(
+    ``!a b region. (m0_non_r_eq  region a b) ==>
+        (a.count =  b.count)/\
+        (a.exception =  b.exception)``,
+    
+    SIMP_TAC std_ss [m0_non_r_eq_def, m0_non_r_eq_def]
+);
+
+val EXISTS_PRE_STATE_lem = prove(``
+! P t seq seq' (i:num) (s:m0_state) (s':m0_state) region .
+	VC region P t /\
+	NEX P t /\
+	  SEP_REFINE (P * SEP_T) $= (STATE m0_proj) s /\
+          m0_non_r_eq region s s' /\ 
+	  rel_sequence (NEXT_REL $= NextStateM0) seq s /\
+	  rel_sequence (NEXT_REL $= NextStateM0) seq' s' /\
+          (seq i).count > (seq 0).count/\
+          ((seq i).count = s.count+t) ==>   
+             ?i'.( ((seq i' ).count < (s.count +t))
+                    /\ ((seq (SUC i'))=(seq i)) 
+                    /\ ((seq' (SUC i'))=(seq' i)))
+``,
+
+    REPEAT STRIP_TAC>> 
+    `
+            ∃i'. (seq i').count < (seq i).count ∧ (seq (i' + 1) = seq i)
+
+    ` by METIS_TAC[ SEQ_EXISTS_PREV_STATE_thm ]>>
+    
+    qexists_tac  `i'`>>
+    rfs [ DECIDE``i' + 1 = SUC i' ``]>>
+    (* parallel run has same prestate lemma *)
+           Cases_on  `i'>=i`>- (
+                `(seq i).count ≤ (seq i').count` by  
+                        METIS_TAC[SEQ_MONO_B, DECIDE ``  (i':num >= i ) <=> (i<= i') `` ]>>
+                `(seq i').count <  (seq i).count` by asm_simp_tac arith_ss[]>>
+                full_simp_tac arith_ss[]
+           )>>
+           Cases_on  `i'+1=i`>-( 
+                fs [DECIDE ``i'+1=SUC i'``]
+           )>>
+           
+(*           `i'< i-1` by DECIDE_TAC>>
+           `i'<= i-1` by DECIDE_TAC>>
+           `i' + 2<= i` by DECIDE_TAC>>
+           `(seq i').count ≤ (seq (i-1)).count` by METIS_TAC[ SEQ_MONO_B]
+           `(seq (i'+2)).count ≤ (seq (i)).count` by METIS_TAC[ SEQ_MONO_B]
+           `   
+                (seq (i'+1)).count < (Next (seq (i'+ 1))).count ∧
+                ((Next (seq (i'+1))).exception = NoException)
+           `by METIS_TAC[NEX_def, DECIDE  ``s.count + t=  t+s.count``]
+
+            `(Next (seq' i')).exception = NoException ` by METIS_TAC[m0_non_r_eq_lem] 
+
+*)
+    `
+           seq' (SUC i') = seq' i
+           
+    ` by cheat>>
+    fs[]
+);
+
+
+
+val FINAL_STATE_EQ_lem = prove(
+``! P t seq seq' (i:num) (s:m0_state) (s':m0_state) region .
+	VC region P t /\
+	NEX P t /\
+               SEP_REFINE (P * SEP_T) $= (STATE m0_proj) s /\
+               m0_non_r_eq region s s' /\ 
+               rel_sequence (NEXT_REL $= NextStateM0) seq  s /\
+               rel_sequence (NEXT_REL $= NextStateM0) seq' s' /\
+               ((seq i).count = s.count+t) ==>   
+                   m0_non_r_eq region (seq i) (seq' i) /\
+                   m0_r_eq region (seq' 0) (seq' i)
+``,
+    REPEAT GEN_TAC>>
+    STRIP_TAC>>
+    (* take care of the case of t=0 *)
+    Tactical.REVERSE ( Cases_on `t>0` ) >- (
+        `t=0` by DECIDE_TAC>>
+         rm_assum  `¬(t > 0)`>>
+         fs []>>
+         cheat
+    )>>
+    `
+                (seq i).count > (seq 0).count 
+
+    ` by ( 
+        `seq 0 = s` by METIS_TAC [rel_sequence_def]>> rfs[] >> 
+        DECIDE_TAC
+    )>>
+    (* there exists a state in the sequance that  *)
+    (*   will transition to a state equal to the  *)
+    (*   final state                              *)
+    `
+             ?i'. ((seq i' ).count < (s.count +t))
+                    /\ ((seq (SUC i'))=(seq i)) 
+                    /\ ((seq' (SUC i'))=(seq' i))
+
+    ` by METIS_TAC[EXISTS_PRE_STATE_lem]>>
+    METIS_TAC[VC_def, EXISTS_PRE_STATE_lem]
+    
+);
+    
+
+val  VC_RUN_EXISTS_lem = prove(
+``! P t seq i s .
+	VC uart_r P t /\
+	NEX P t /\
+	  SEP_REFINE (P * SEP_T) $= (STATE m0_proj) s /\
+	  rel_sequence (NEXT_REL $= NextStateM0) seq s /\
+	  (seq i).count < s.count + t ==> 
+            ! z_i.(
+              m0_non_r_eq uart_r z_i (seq i)==>
+                ? z_0.
+                  !seq_z. (rel_sequence (NEXT_REL $= NextStateM0) seq_z z_0) ==>
+                        ((seq_z i) = z_i) /\
+                          m0_non_r_eq uart_r s z_0 /\
+                          m0_r_eq uart_r z_0 z_i
+            )
+``,
+    
+    REPEAT STRIP_TAC>>
+    EXISTS_TAC ``s with <|MEM := (\x. if (x IN uart_r) 
+                                         then (z_i.MEM x)
+                                         else (s.MEM x)) |>``>>
+    REPEAT STRIP_TAC>>
+    `m0_non_r_eq uart_r s (s with MEM := (λx. if x ∈ uart_r then z_i.MEM x else s.MEM x)) /\
+     m0_r_eq uart_r (s with MEM := (λx. if x ∈ uart_r then z_i.MEM x else s.MEM x)) z_i` by (
+           SIMP_TAC (std_ss++pred_setLib.PRED_SET_ss) [
+                m0Theory.m0_state_accfupds,m0_non_r_eq_def, m0_r_eq_def, mem_eq_def
+           ]
+    )>>
+    Q.ABBREV_TAC `z_0=(s with MEM := (λx. if x ∈ uart_r then z_i.MEM x else s.MEM x))`>>
+    (MP_TAC o
+        Q.SPECL [`P`, `(seq (i:num)).count-s.count`, `seq`, `seq_z`, `i`, `s`, `z_0`, `uart_r`])
+        FINAL_STATE_EQ_lem >>
+    (* apply weakening *)
+    
+    `s.count <= (seq i).count` by METIS_TAC[SEQ_MONO_B, DECIDE ``0n<=i:num``,rel_sequence_def ]>>
+    `((seq i).count = s.count + ((seq i).count − s.count)) ` by DECIDE_TAC>>
+    `((seq i).count -s.count) <= t` by DECIDE_TAC>>
+    `VC uart_r P ((seq i).count -s.count)∧ NEX P ((seq i).count -s.count)` by METIS_TAC[VC_WEAKEN_lem, NEX_WEAKEN_lem]>>
+        ASM_SIMP_TAC std_ss[]>>
+	METIS_TAC[m0_r_eq_trans_thm, m0_r_eq_antisym_thm,
+                  m0_non_r_eq_trans_thm, m0_non_r_eq_antisym_thm,
+                  eq_lem,rel_sequence_def]
+);
+
+val   VC_NIT_STEP_thm = store_thm("VC_NIT_STEP_thm",
+``  ! P t s seq i.
+	VC uart_r P t /\
+	NEX P t /\
+	SEP_REFINE (P * SEP_T) $= (STATE m0_proj) s /\
+	rel_sequence (NEXT_REL $= NextStateM0) seq s /\
+	(seq i).count < s.count + t ==> NIT_STEP uart_r (seq i)``,
+
+    REPEAT STRIP_TAC >>
+    SIMP_TAC std_ss [NIT_STEP_thm]>>
+    GEN_TAC>>
+    rename1 `m0_non_r_eq uart_r (seq i) z_i`>>
+    STRIP_TAC>>
+     `              
+            ∃z_0.
+                ∀seq_z.
+                    rel_sequence (NEXT_REL $= NextStateM0) seq_z z_0 ⇒
+                    (seq_z i = z_i)/\ m0_non_r_eq uart_r s z_0 /\ m0_r_eq uart_r z_0 z_i
+
+     `by METIS_TAC[ VC_RUN_EXISTS_lem, m0_non_r_eq_antisym_thm]>>
+
+
+     `
+              ?seq_z . rel_sequence (NEXT_REL $= NextStateM0) seq_z z_0
+
+     ` by( METIS_TAC[SEQUENCE_EXISTS_THM])>>
+
+     `              
+                     (seq_z i = z_i)/\ m0_non_r_eq uart_r s z_0/\m0_r_eq uart_r z_0 z_i
+     ` by METIS_TAC[]>>
+     rm_assum `∀seq_z._`>>
+     `              
+          m0_non_r_eq uart_r (seq (SUC i)) (seq_z (SUC i)) ∧
+          m0_r_eq uart_r (seq_z 0) (seq_z (SUC i))
+     `   by METIS_TAC[VC_def] >>
+   `(seq(SUC i) = Next (seq(i)))` by  (METIS_TAC[NEX_thm])>>
+   `(seq_z(SUC i) = Next (seq_z(i)))` by(
+        (* a step must have taken place between (seq_z i) and i+1 
+           since the count between them has increesed *) 
+	`(seq_z(i)).count < (seq_z(SUC i)).count ` by
+	    METIS_TAC[NEX_thm,  m0_non_r_eq_def]>>
+	Q.PAT_X_ASSUM `rel_sequence (NEXT_REL $= NextStateM0) seq_z s_0` 
+	    (MP_TAC o Q.SPEC `i` o 
+	    SIMP_RULE (std_ss++LET_ss)[
+		rel_sequence_def, PULL_EXISTS,NEXT_REL_EQ,
+		NextStateM0_def, PULL_FORALL])>>
+         IF_CASES_TAC >-  (METIS_TAC[] )>>
+	 STRIP_TAC >> FULL_SIMP_TAC arith_ss[]
+    )>>
+    rm_assum `VC _ _ _`>>
+    rm_assum `NEX  _ _`>>
+    METIS_TAC[m0_r_eq_trans_thm,m0_r_eq_antisym_thm, rel_sequence_def]
+    
+);
+ 
+
+
+(* cosim *)
+val COSIM'_def = Define `COSIM' P t = ! s s' seq seq' i.
+    ((SEP_REFINE (P * SEP_T) ($=) (STATE m0_proj) s) /\
+    rel_sequence (NEXT_REL $= NextStateM0) seq  s /\
+    rel_sequence (NEXT_REL $= NextStateM0U) seq' s' /\
+    m0u_m0_non_r_eq uart_r s' s /\ ((seq i).count < s.count + t) )==>
+        m0u_m0_non_r_eq uart_r (m0u_Next (seq' i)) (Next (seq i)) /\
+        m0u_r_eq uart_r (seq' i)  (m0u_Next (seq' i))`;
+
+val COSIM_def = Define `COSIM P t = ! s s' seq seq' i.
+    ((SEP_REFINE (P * SEP_T) ($=) (STATE m0_proj) s) /\
+    rel_sequence (NEXT_REL $= NextStateM0) seq  s /\
+    rel_sequence (NEXT_REL $= NextStateM0U) seq' s' /\
+    m0u_m0_non_r_eq uart_r s' s /\ ((seq i).count < s.count + t) )==>
+        m0u_m0_non_r_eq uart_r (seq' (SUC i)) (seq (SUC i)) /\
+        m0u_r_eq uart_r (seq' i)  (seq' (SUC i))`;
+
+val cosim_def = Define `cosim P c t = COSIM ((CODE_POOL m0_instr c) * P  ) t`;
 
 
 val LEM = prove(
@@ -168,6 +381,7 @@ val LEM = prove(
 );
 
 
+
 val LEM1 = prove(
     ``!a b region. (m0u_m0_non_r_eq  region a b) ==>
         (((FST o FST) a).count =  b.count)/\
@@ -176,9 +390,8 @@ val LEM1 = prove(
     SIMP_TAC std_ss [m0u_m0_non_r_eq_def, m0_non_r_eq_def]
 );
 
-
-val NIT_COSIM'_thm = Q.store_thm ("NIT_COSIM'_thm",
-    `!P t.  ((NIT uart_r P t) /\ (NEX P t)) ==> (COSIM' P t)`,
+val VC_COSIM'_thm = Q.prove (
+    `!P t.  ((VC uart_r P t) /\ (NEX P t)) ==> (COSIM' P t)`,
     SIMP_TAC std_ss [ COSIM'_def, PULL_FORALL]>>
     REPEAT GEN_TAC>>
     STRIP_TAC>>
@@ -188,7 +401,7 @@ val NIT_COSIM'_thm = Q.store_thm ("NIT_COSIM'_thm",
         STRIP_TAC>>
         `((seq 0).count < (Next (seq 0)).count) ∧( (Next (seq 0) = seq (SUC 0)))` by
             METIS_TAC[NEX_thm]>>
-        `NIT_STEP uart_r (seq 0)` by METIS_TAC[NIT_NIT_STEP_thm]>>
+        `NIT_STEP uart_r (seq 0)` by METIS_TAC[VC_NIT_STEP_thm]>>
         METIS_TAC[rel_sequence_def, AXI, m0u_r_eq_antisym_thm]
     )>>
     STRIP_TAC >>
@@ -200,7 +413,7 @@ val NIT_COSIM'_thm = Q.store_thm ("NIT_COSIM'_thm",
     (Next (seq i) = seq (SUC i))` by METIS_TAC[NEX_thm]>>
     ` (seq (SUC i)).count < (Next (seq (SUC i))).count ∧
     (Next (seq (SUC i)) = seq (SUC(SUC i)))` by METIS_TAC[NEX_thm]>>
-    `NIT_STEP uart_r (seq (SUC i) )` by METIS_TAC[NIT_NIT_STEP_thm]>>
+    `NIT_STEP uart_r (seq (SUC i) )` by METIS_TAC[VC_NIT_STEP_thm]>>
     `m0u_Next (seq' i) =  (seq' (SUC i))` by (
         ` ((FST ∘ FST) (m0u_Next (seq' i))).exception = NoException` by METIS_TAC[LEM1,NEX_def]>>
         `if ∃x. NEXT_REL $= NextStateM0U (seq' i) x then
@@ -213,10 +426,11 @@ val NIT_COSIM'_thm = Q.store_thm ("NIT_COSIM'_thm",
 );
 
 
-val NIT_COSIM''_thm = Q.prove(`!P t.  ((NIT uart_r P t) /\ (NEX P t)) ==> (COSIM'' P t)`,
-    fs[COSIM''_def, PULL_FORALL]>>
+(* Theorem 2 in repport *)
+val VC_COSIM_thm = Q.prove(`!P t.  ((VC uart_r P t) /\ (NEX P t)) ==> (COSIM P t)`,
+    fs[COSIM_def, PULL_FORALL]>>
     REPEAT gen_tac>> strip_tac >>strip_tac>>
-    `COSIM' P t` by fs[NIT_COSIM'_thm]>>
+    `COSIM' P t` by fs[VC_COSIM'_thm]>>
     ` m0u_m0_non_r_eq uart_r (m0u_Next (seq' i)) (Next (seq i)) ∧
              m0u_r_eq uart_r (seq' i) (m0u_Next (seq' i))` by ( 
         fs[COSIM'_def]>> METIS_TAC[]
@@ -236,15 +450,20 @@ val NIT_COSIM''_thm = Q.prove(`!P t.  ((NIT uart_r P t) /\ (NEX P t)) ==> (COSIM
     fs[]
 );
 
-val NIT_COSIM_thm = Q.store_thm ("NIT_COSIM_thm",
-    `!P t.  ((NIT uart_r P t) /\ (NEX P t)) ==> (COSIM P t)`,
-                           (* use NIT_COSIM''_thm *)
+val FINAL_STATE_EQ_thm = Q.store_thm ("VC_COSIM_thm",
+    `!P t.  ((VC uart_r P t) /\ (NEX P t)) ==> ! s s' seq seq' i.
+    ((SEP_REFINE (P * SEP_T) ($=) (STATE m0_proj) s) /\
+    rel_sequence (NEXT_REL $= NextStateM0) seq  s /\
+    rel_sequence (NEXT_REL $= NextStateM0U) seq' s' /\
+    m0u_m0_non_r_eq uart_r s' s /\ ((seq i).count = s.count + t) )==>
+        m0u_m0_non_r_eq uart_r (seq' ( i)) (seq ( i)) /\
+        m0u_r_eq uart_r (seq' 0)  (seq' ( i))`,
     cheat);
      
 (* 
-`!P t.  ((NIT uart_r P t) /\ (NEX P t)) ==> (COSIM2 P t)`,
+`!P t.  ((VC uart_r P t) /\ (NEX P t)) ==> (COSIM2 P t)`,
         REPEAT STRIP_TAC >>
-       `COSIM P t ` by fs[ NIT_COSIM_thm]>> 
+       `COSIM P t ` by fs[ VC_COSIM_thm]>> 
        fs[COSIM2_def] >> 
         REPEAT GEN_TAC >>
              
